Use lists, not sets

src/defs/fv.lean
@@ -2,19 +2,19 @@ import defs.syntax
 import defs.var
 
 @[reducible]
-def fv (e: exp): set var :=
+def fv (e: exp): list var :=
   exp.rec_on e
   -- int
-  (fun _, ∅)
+  (fun _, [])
   -- true
-  ∅
+  []
   -- false
-  ∅
+  []
   -- if_
-  (fun _ _ _ s1 s2 s3, s1 ∪ s2 ∪ s3)
+  (fun _ _ _ s1 s2 s3, s1 ++ (s2 ++ s3))
   -- var
   (fun x, {x})
   -- fn
-  (fun x _ _ s, s \ {x})
+  (fun x _ _, list.filter (fun y, x ≠ y))
   -- app
-  (fun _ _ s1 s2, s1 ∪ s2)
+  (fun _ _ s1 s2, s1 ++ s2)
